---
aliases: 
tags:
  - batch/math
  - batch/school/class/ma110
---
Sam Tang
Dr. Hunter
Abstract Algebra
2023-10-02
# Pre-Work Problems 73 Through 77 MA-110

> [!problem] Problem 5.73
> Let $H$ be a subgroup of a group $G$. Prove that $H\trianglelefteq G$ if and only if the following condition holds: for all $h \in H$ and for all $g \in G$, $ghg^{-1}$ is in $H$.

Let $H$ be a subgroup of a group $G$. First, suppose $H\trianglelefteq G$ and let $h \in H$ and $g \in G$. Because $H\trianglelefteq G$, there exists some $h' \in H$ such that $gh=h'g$. Thus,
$$
ghg^{-1} =h'g g^{-1} = h' \in  H.
$$

Now, suppose for all $h \in H$ and $g \in G$, $ghg^{-1} \in H$. Let $g_{0} \in G$ be given, and suppose $x \in g_{0}H$. Then $x=g_{0}h$ for some $h \in H$. Right multiplying by $g_{0}^{-1}g_{0}$ yields
$$
\begin{align}
x(g_{0}^{-1}g_{0}) &= g_{0}h(g_{0}^{-1}g_{0}) \\
x&= (g_{0}hg_{0}^{-1})g_{0} \\
x &= h'g_{0}. && \text{for some } h' \in  H
\end{align}
$$
Therefore, $x \in Hg_{0}$ and $g_{0}H\subseteq Hg_{0}$. We can argue similarly to show $Hg_{0}\subseteq g_{0}H$. Therefore $g_{0}H=Hg_{0}$ and $H\trianglelefteq G$.

> [!problem] Problem 5.74
> Suppose that $H$ is a normal subgroup of group $G$. Let $a,b \in G$ and define $X=aH$ and $Y=bH$. Prove that $XY=(ab)H$.

^e12182

Let $H\trianglelefteq G$ with $a,b \in G$ and define $X=aH$ and $Y=bH$. In [[Pre-Work Problems 69 Through 72 MA-110#^fc2739|Problem 72]] we showed $XY\subseteq(ab)H$.

Suppose that $n \in (ab)H$. Then, for some $h \in H$, $n =(ab)h$. Note this is equivalent to $a(bh)$. $bh \in bH=Y$ by definition, and $a \in aH$, so $a(bh) \in XY$. Thus, $(ab)H \subseteq XY$ and $XY=(ab)H$.

<div class="page-break" style="page-break-after: always;"></div> 

> [!problem] Problem 5.75
> Give an example to show that the hypothesis that $H\trianglelefteq G$ is needed in [[#^e12182|Problem 74]]. That is, find an example of a group and a subgroup where the product of two cosets fails to be a coset.

Consider the group $D_{3}$ with subgroup $H=\{ (1), (1\ 2) \}$. If we consider
$$
((1\ 2\ 3)H)H= \{ (1\ 2\ 3), (1\ 3) \}\{ (1), (1\ 2) \}=\{ (1), (1\ 2), (1\ 3), (1\ 2\ 3) \}.
$$
The resulting product cannot be a coset, it has order four while $H$ has order two.

> [!problem] Problem 5.76
> Let $H$ be a normal subgroup of a group $G$. Prove that the set $G/H$ is a group under coset multiplication.

Let $H$ be a normal subgroup of a group $G$, and consider the set $G/H$ under coset multiplication.

Let $A,B,C \in G/H$.
$$
\begin{align}
(AB)C = \{ ab : a \in  A, b \in  B \}\{ c: c \in  C \}&=\{ (ab)c : a \in  A, b \in  B, c \in  C\} \\
A(BC) = \{ a : a \in  A \}\{ bc: b \in  B, c \in  C \}&=\{ a(bc) : a \in  A, b \in  B, c \in  C\} \\
&= \{ (ab)c: a \in  A, b \in  B, c \in  C \}.
\end{align}
$$
Therefore, $G/H$ is associative.

By [[#^e12182|Problem 74]], $G/H$ is closed under multiplication and therefore a valid binary operation.

Let $A \in G/H$. We can represent $A=aH$ and $H=eH$ where $a \in G$ and $e$ is the identity of $G$. Problem 74 states $AH=(aH)(eH)=(ae)H=aH=A$. Thus, by the test for inverses, $H$ is the identity of $G/H$.

Let $A \in G/H$. By definition, we can represent $A=aH$, where $a \in G$. By Problem 74, $(aH)(a^{-1}H)=(aa^{-1})H=H$. Therefore, every element of $G/H$ has an inverse.

Thus, $G/H$ under coset multiplication satisfies all of the criteria of a group.

> [!problem] Problem 5.77
> Let $G=\mathbb{Z}_{4}\times \mathbb{Z}_{6}$, and let $H$ be the cyclic subgroup generated by $(2,2)$. That is, $H=\langle (2,2)\rangle$. Notice that $H\trianglelefteq G$ since $G$ is abelian. Give the group table for $G/H$. What well-known group is $G/H$ isomorphic to?

Let $G=\mathbb{Z}_{4}\times \mathbb{Z}_{6}$, and let $H$ be the cyclic subgroup generated by $(2,2)$.
$$
H=\{ (2,2), (0,4), (2,0), (0,2), (2,4), (0,0) \}
$$
Because $H$ has order $6$, there must be four cosets. Thus,
$$
G/H=\{ H, (1,0)H,(1,1)H, (0,1)H\}.
$$

|          | $H$      | $(1,0)H$ | $(1,1)H$ | $(0,1)H$ |
| -------- | -------- | -------- | -------- | -------- |
| $H$      | $H$      | $(1,0)H$ | $(1,1)H$ | $(0,1)H$ |
| $(1,0)H$ | $(1,0)H$ | $H$      | $(0,1)H$ | $(1,1)H$ |
| $(1,1)H$ | $(1,1)H$ | $(0,1)H$ | $H$ | $(1,2)H$ |
| $(0,1)H$ | $(0,1)H$ | $(1,1)H$ | $(1,0)H$ | $H$ |

$G/H$ is isomorphic to $\mathbb{Z}_{2}\times \mathbb{Z}_{2}$.