---
aliases: 
tags:
  - batch/school/class/ma110
  - batch/math
type: Problem
related:
  - "[[Problem 6.92 MA-110]]"
---
# Problem 6.93 MA-110

> [!problem] Problem 6.93
> Let $R$ be a ring with unity, and let $r \in R$. Let $-1$ denote the additive inverse of $1$. Prove that $-1 \cdot r=-r$. (That is, show that $-1 \cdot r$ is the additive inverse of $r$.)

Let $R$ be a ring with unity, and let $r \in R$.
$$
\begin{align}
r + (-1 \cdot r) &= (1 + (-1))r && \text{multiplicative associativity} \\
&= (0)r && \text{definition of additive inverses} \\
&= 0. && \text{Problem 92}
\end{align}
$$
Therefore, $r$ and $-1 \cdot r$ are additive inverses and $-1 \cdot r=-r$. 